Contexts.thy
@@ -13,7 +13,7 @@ begin
 lemma medial_subset:
   "length i = Arity t \<Longrightarrow>
    Arity t = Arity t' \<Longrightarrow>
-   set (Guard t') \<subseteq> set (Guard t) \<Longrightarrow>
+   set (Guards t') \<subseteq> set (Guards t) \<Longrightarrow>
    can_take_transition t i r \<Longrightarrow>
    can_take_transition t' i r"
   by (simp add: can_take_transition_def can_take_def apply_guards_subset)
@@ -22,25 +22,26 @@ definition posterior_separate :: "nat \<Rightarrow> vname gexp list \<Rightarrow
   "posterior_separate a g u i r = (if can_take a g i r then Some (apply_updates u (join_ir i r) r) else None)"
 
 definition posterior :: "transition \<Rightarrow> inputs \<Rightarrow> registers \<Rightarrow> registers option" where
-  "posterior t i r = posterior_separate (Arity t) (Guard t) (Updates t) i r"
+  "posterior t i r = posterior_separate (Arity t) (Guards t) (Updates t) i r"
 
 definition subsumes :: "transition \<Rightarrow> registers \<Rightarrow> transition \<Rightarrow> bool" where
   "subsumes t2 r t1 = (Label t1 = Label t2 \<and> Arity t1 = Arity t2 \<and>
                        (\<forall>i. can_take_transition t1 i r \<longrightarrow> can_take_transition t2 i r) \<and>
                        (\<forall>i. can_take_transition t1 i r \<longrightarrow>
                             apply_outputs (Outputs t1) (join_ir i r) = apply_outputs (Outputs t2) (join_ir i r)) \<and>
-                       (\<forall>p1 p2 i. posterior_separate (Arity t1) (Guard t1) (Updates t2) i r = Some p2 \<longrightarrow>
-                                  posterior_separate (Arity t1) (Guard t1) (Updates t1) i r = Some p1 \<longrightarrow>
+                       (\<forall>p1 p2 i. posterior_separate (Arity t1) (Guards t1) (Updates t2) i r = Some p2 \<longrightarrow>
+                                  posterior_separate (Arity t1) (Guards t1) (Updates t1) i r = Some p1 \<longrightarrow>
                                   (\<forall>P r'. (p1 $ r' = None) \<or> (P (p2 $ r') \<longrightarrow> P (p1 $ r'))))
                       )"
 
-lemma subsumption: 
+lemma subsumption:
+
   "(Label t1 = Label t2 \<and> Arity t1 = Arity t2) \<Longrightarrow>
    (\<forall>i. can_take_transition t1 i r \<longrightarrow> can_take_transition t2 i r) \<Longrightarrow>
    (\<forall>i. can_take_transition t1 i r \<longrightarrow>
         apply_outputs (Outputs t1) (join_ir i r) = apply_outputs (Outputs t2) (join_ir i r)) \<Longrightarrow>
-   (\<forall>p1 p2 i. posterior_separate (Arity t1) (Guard t1) (Updates t2) i r = Some p2 \<longrightarrow>
-              posterior_separate (Arity t1) (Guard t1) (Updates t1) i r = Some p1 \<longrightarrow>
+   (\<forall>p1 p2 i. posterior_separate (Arity t1) (Guards t1) (Updates t2) i r = Some p2 \<longrightarrow>
+              posterior_separate (Arity t1) (Guards t1) (Updates t1) i r = Some p1 \<longrightarrow>
               (\<forall>P r'. (p1 $ r' = None) \<or> (P (p2 $ r') \<longrightarrow> P (p1 $ r')))) \<Longrightarrow>
    subsumes t2 r t1"
   by (simp add: subsumes_def)
@@ -51,18 +52,32 @@ lemma bad_guards:
   by (simp add: subsumes_def)
 
 lemma inconsistent_updates:
-  "\<exists>p2 p1. (\<exists>i. posterior_separate (Arity t1) (Guard t1) (Updates t2) i r = Some p2 \<and>
-                posterior_separate (Arity t1) (Guard t1) (Updates t1) i r = Some p1) \<and>
+  "\<exists>p2 p1. (\<exists>i. posterior_separate (Arity t1) (Guards t1) (Updates t2) i r = Some p2 \<and>
+                posterior_separate (Arity t1) (Guards t1) (Updates t1) i r = Some p1) \<and>
            (\<exists>r' P. P (p2 $ r') \<and> (\<exists>y. p1 $ r' = Some y) \<and> \<not> P (p1 $ r')) \<Longrightarrow>
     \<not> subsumes t2 r t1"
   by (metis (no_types, hide_lams) option.simps(3) subsumes_def)
 
-lemma bad_outputs: "\<exists>i. can_take_transition t1 i r \<and> apply_outputs (Outputs t1) (join_ir i r) \<noteq> apply_outputs (Outputs t2) (join_ir i r) \<Longrightarrow>
+lemma bad_outputs:
+"\<exists>i. can_take_transition t1 i r \<and> apply_outputs (Outputs t1) (join_ir i r) \<noteq> apply_outputs (Outputs t2) (join_ir i r) \<Longrightarrow>
  \<not> subsumes t2 r t1"
   by (simp add: subsumes_def)
 
-lemma transition_subsumes_self: "subsumes t c t"
+lemma transition_subsumes_self:
+"subsumes t c t"
   by (simp add: subsumes_def)
+
+primrec accepting_sequence :: "transition_matrix \<Rightarrow> cfstate \<Rightarrow> registers \<Rightarrow> trace \<Rightarrow> (transition \<times> cfstate \<times> outputs \<times> registers) list \<Rightarrow> (transition \<times> cfstate \<times> outputs \<times> registers) list option" where
+  "accepting_sequence _ _ r [] obs = Some (rev obs)" |
+  "accepting_sequence e s r (a#t) obs = (let
+    poss = possible_steps e s r (fst a) (snd a);
+    accepting = ffilter (\<lambda>(s', T). accepts e s' (apply_updates (Updates T) (join_ir (snd a) r) r) t) poss in
+    case random_member accepting of
+    None \<Rightarrow> None |
+    Some (s', T) \<Rightarrow> let
+      r' = (apply_updates (Updates T) (join_ir (snd a) r) r) in
+      accepting_sequence e s' r' t ((T, s', (apply_outputs (Outputs T) (join_ir (snd a) r)), r')#obs)
+  )"
 
 definition posterior_sequence :: "transition_matrix \<Rightarrow> cfstate \<Rightarrow> registers \<Rightarrow> trace \<Rightarrow> registers option" where
   "posterior_sequence e s r t = (case accepting_sequence e s r t [] of
@@ -77,37 +92,34 @@ definition posterior_sequence :: "transition_matrix \<Rightarrow> cfstate \<Righ
 abbreviation anterior_context :: "transition_matrix \<Rightarrow> trace \<Rightarrow> registers option" where
   "anterior_context e t \<equiv> posterior_sequence e 0 <> t"
 
-lemma anterior_context_empty: "anterior_context e [] = Some <>"
+lemma anterior_context_empty:
+"anterior_context e [] = Some <>"
   by (simp add: posterior_sequence_def)
 
-lemma posterior_sequence_implies_accepting_sequence: "posterior_sequence e s d t = Some ca \<Longrightarrow> accepting_sequence e s d t [] \<noteq> None"
+lemma posterior_sequence_implies_accepting_sequence:
+"posterior_sequence e s d t = Some ca \<Longrightarrow> accepting_sequence e s d t [] \<noteq> None"
   apply (simp add: posterior_sequence_def)
   by (cases "accepting_sequence e s d t []", auto)
 
-lemma accepting_sequence_accepts: "accepting_sequence e s d t [] = Some y \<Longrightarrow> accepts e s d t"
-proof(induct t arbitrary: d)
+lemma accepting_sequence_accepts:
+"accepting_sequence e s r t [] = Some y \<Longrightarrow> accepts e s r t"
+proof(induct t arbitrary: r)
   case Nil
   then show ?case
     by (simp add: accepts.base)
 next
-  case (Cons a t)
+  case (Cons a ts)
   then show ?case
-    apply (simp add: Let_def)
-    apply (case_tac "ffilter (\<lambda>(s', T). accepts e s' (apply_updates (Updates T) (join_ir (snd a) d) d) t)
-         (possible_steps e s d (fst a) (snd a)) = {||}")
+    apply (cases a)
+      apply simp
+      apply (case_tac "random_member
+              (ffilter (\<lambda>(s', T). accepts e s' (apply_updates (Updates T) (join_ir b r) r) ts) (possible_steps e s r aa b))")
      apply simp
-    apply simp
-    apply (case_tac "SOME x.
-             x |\<in>| possible_steps e s d (fst a) (snd a) \<and>
-             (case x of (s', T) \<Rightarrow> accepts e s' (apply_updates (Updates T) (join_ir (snd a) d) d) t)")
-    apply (simp add: Let_def)
-    apply (case_tac a)
-    apply simp
-    apply (rule accepts.step)
-    by fastforce
+    using accepts.step random_member_Some by fastforce
 qed
 
-lemma posterior_sequence_accepts: "posterior_sequence e s d t = Some ca \<longrightarrow> accepts e s d t"
+lemma posterior_sequence_accepts:
+"posterior_sequence e s d t = Some ca \<longrightarrow> accepts e s d t"
   using posterior_sequence_implies_accepting_sequence[of e s d t ca]
   apply simp
   apply clarify
@@ -115,10 +127,12 @@ lemma posterior_sequence_accepts: "posterior_sequence e s d t = Some ca \<longri
   using accepting_sequence_accepts
   by auto
 
-lemma anterior_context_accepts: "\<exists>c. anterior_context e p = Some c \<Longrightarrow> accepts_trace e p"
+lemma anterior_context_accepts:
+"\<exists>c. anterior_context e p = Some c \<Longrightarrow> accepts_trace e p"
   using posterior_sequence_accepts by blast
 
-lemma posterior_sequence_gives_accept: "posterior_sequence e s d t \<noteq> None \<Longrightarrow> accepts e s d t"
+lemma posterior_sequence_gives_accept:
+"posterior_sequence e s d t \<noteq> None \<Longrightarrow> accepts e s d t"
   using option.discI posterior_sequence_accepts by auto
 
 lemma accepting_sequence_posterior_sequence_not_none:
@@ -131,69 +145,76 @@ lemma accepting_sequence_posterior_sequence_not_none:
   apply (case_tac "last a")
   by simp
 
-lemma posterior_sequence_none_accepting_sequence_none: "(posterior_sequence e s d t = None) = (accepting_sequence e s d t [] = None)"
+lemma posterior_sequence_none_accepting_sequence_none:
+"(posterior_sequence e s d t = None) = (accepting_sequence e s d t [] = None)"
   apply standard
   using accepting_sequence_posterior_sequence_not_none apply blast
   by (simp add: posterior_sequence_def)
 
-lemma rejects_gives_no_accepting_sequence: "\<forall>s d. \<not>accepts e s d t \<longrightarrow> accepting_sequence e s d t [] = None"
-proof(induct t)
+lemma rejects_gives_no_accepting_sequence: "rejects e s r t \<Longrightarrow> accepting_sequence e s r t [] = None"
+proof(induct t arbitrary: s r)
   case Nil
   then show ?case
     by (simp add: accepts.base)
 next
   case (Cons a t)
   then show ?case
-    apply clarify
     apply (cases a)
-    apply (simp only: trace_reject_2)
-    apply (simp add: Let_def)
-    apply (case_tac "SOME x.
-                x |\<in>| possible_steps e s d aa b \<and>
-                (case x of (s', T) \<Rightarrow> accepts e s' (apply_updates (Updates T) (join_ir b d) d) t)")
     apply simp
-    by fastforce
+    apply (case_tac "random_member
+              (ffilter (\<lambda>(s', T). accepts e s' (apply_updates (Updates T) (join_ir b r) r) t) (possible_steps e s r aa b))")
+     apply simp
+    using accepts.step random_member_Some by fastforce
 qed
 
-lemma rejects_gives_no_posterior_sequence: "\<not>accepts e s d t \<Longrightarrow> posterior_sequence e s d t = None"
-  by (simp add: posterior_sequence_def rejects_gives_no_accepting_sequence)
+lemma rejects_gives_no_posterior_sequence: "rejects e s d t \<Longrightarrow> posterior_sequence e s d t = None"
+  using posterior_sequence_gives_accept by blast
 
-lemma no_accepting_sequence_rejected: "\<forall>d s seq. accepting_sequence e s d t seq = None \<longrightarrow> \<not> accepts e s d t"
-proof(induct t)
+lemma no_accepting_sequence_rejected: "accepting_sequence e s d t seq = None \<longrightarrow> rejects e s d t"
+proof(induct t arbitrary: s d seq)
   case Nil
   then show ?case
     by simp
 next
   case (Cons a t)
   then show ?case
+    apply (cases a)
+    apply simp
+    apply (case_tac "random_member
+              (ffilter (\<lambda>(s', T). accepts e s' (apply_updates (Updates T) (join_ir b d) d) t) (possible_steps e s d aa b))")
+     apply simp
+     apply clarify
+     apply (rule accepts.cases)
+       apply simp
+      apply simp
+     apply auto[1]
+    apply simp
+    apply (case_tac aaa)
     apply clarify
     apply (rule accepts.cases)
       apply simp
      apply simp
     apply clarify
-    apply (simp add: Let_def)
-    apply (case_tac "ffilter (\<lambda>(s', T). accepts e s' (apply_updates (Updates T) (join_ir i da) da) t) (possible_steps e sa da l i) = {||}")
-     apply auto[1]
     apply simp
-    apply (case_tac "SOME x.
-                x |\<in>| possible_steps e sa da l i \<and>
-                (case x of (s', T) \<Rightarrow> accepts e s' (apply_updates (Updates T) (join_ir i da) da) t)")
-    apply (simp add: Let_def)
-    by (metis (no_types, lifting) case_prodD case_prodI someI_ex)
+    by (metis (mono_tags, lifting) case_prodD ffmember_filter random_member_Some)
 qed
 
-lemma no_posterior_sequence_reject: "posterior_sequence e s d t = None \<Longrightarrow> \<not>accepts e s d t"
+lemma no_posterior_sequence_reject:
+"posterior_sequence e s d t = None \<Longrightarrow> \<not>accepts e s d t"
   apply (simp add: posterior_sequence_none_accepting_sequence_none)
   using no_accepting_sequence_rejected
   by blast
 
-lemma accepts_gives_context: "\<forall>s d. accepts e s d t \<longrightarrow> (\<exists>c. posterior_sequence e s d t = Some c)"
+lemma accepts_gives_context:
+"\<forall>s d. accepts e s d t \<longrightarrow> (\<exists>c. posterior_sequence e s d t = Some c)"
   using no_posterior_sequence_reject by blast
 
-lemma accepts_trace_gives_context: "accepts_trace e p \<Longrightarrow> (\<exists>c. anterior_context e p = Some c)"
+lemma accepts_trace_gives_context:
+"accepts_trace e p \<Longrightarrow> (\<exists>c. anterior_context e p = Some c)"
   using accepts_gives_context by auto
 
-lemma accepts_trace_anterior_not_none: "accepts_trace e p \<Longrightarrow> anterior_context e p \<noteq> None"
+lemma accepts_trace_anterior_not_none:
+"accepts_trace e p \<Longrightarrow> anterior_context e p \<noteq> None"
   using accepts_trace_gives_context by blast
 
 lemma no_choice_no_subsumption:
@@ -204,7 +225,8 @@ lemma no_choice_no_subsumption:
   \<not> subsumes t c t'"
   by (meson bad_guards can_take_def can_take_transition_def choice_def)
 
-lemma subsumption_def_alt: "subsumes t1 c t2 = (Label t2 = Label t1 \<and>
+lemma subsumption_def_alt:
+"subsumes t1 c t2 = (Label t2 = Label t1 \<and>
     Arity t2 = Arity t1 \<and>
     (\<forall>i. can_take_transition t2 i c \<longrightarrow> can_take_transition t1 i c) \<and>
     (\<forall>i. can_take_transition t2 i c \<longrightarrow> apply_outputs (Outputs t2) (join_ir i c) = apply_outputs (Outputs t1) (join_ir i c)) \<and>
@@ -215,7 +237,8 @@ lemma subsumption_def_alt: "subsumes t1 c t2 = (Label t2 = Label t1 \<and>
   apply (simp add: subsumes_def posterior_separate_def can_take_transition_def[symmetric])
   by blast
 
-lemma subsumes_update_equality: "subsumes t1 c t2 \<Longrightarrow> (\<forall>i. can_take_transition t2 i c \<longrightarrow>
+lemma subsumes_update_equality:
+"subsumes t1 c t2 \<Longrightarrow> (\<forall>i. can_take_transition t2 i c \<longrightarrow>
          (\<forall>r'.
              ((apply_updates (Updates t1) (join_ir i c) c $ r') = (apply_updates (Updates t2) (join_ir i c) c $ r')) \<or>
              apply_updates (Updates t2) (join_ir i c) c $ r' = None))"
@@ -226,7 +249,8 @@ lemma subsumes_update_equality: "subsumes t1 c t2 \<Longrightarrow> (\<forall>i.
   apply (erule_tac x=r' in allE)
   by auto
 
-lemma subsumption_def_alt2: "subsumes t1 c t2 = (Label t2 = Label t1 \<and>
+lemma subsumption_def_alt2:
+"subsumes t1 c t2 = (Label t2 = Label t1 \<and>
     Arity t2 = Arity t1 \<and>
     (\<forall>i. can_take_transition t2 i c \<longrightarrow> can_take_transition t1 i c) \<and>
     (\<forall>i. can_take_transition t2 i c \<longrightarrow> apply_outputs (Outputs t2) (join_ir i c) = apply_outputs (Outputs t1) (join_ir i c)) \<and>
