Transition.thy
@@ -1,6 +1,10 @@
 theory Transition
 imports GExp
 begin
+section\<open>Transitions\<close>
+text\<open>Here we define the transitions which make up EFSMs. As per \cite{foster2018}, each transitions
+has a label and an arity and optionally, guards, outputs, and Updates. To implement this, we use
+the record type such that each component of the transition can be accessed.\<close>
 
 type_synonym label = String.literal
 type_synonym arity = nat
@@ -8,15 +12,16 @@ type_synonym guard = "vname gexp"
 type_synonym inputs = "value list"
 type_synonym outputs = "value option list"
 type_synonym output_function = "vname aexp"
-type_synonym update_function = "(nat \<times> vname aexp)"
+type_synonym update_functions = "(nat \<times> vname aexp) list"
+type_synonym update_function = "nat \<times> vname aexp"
 
 text_raw\<open>\snip{transitiontype}{1}{2}{%\<close>
 record transition =
   Label :: String.literal
   Arity :: nat
-  Guard :: "guard list"
+  Guards :: "guard list"
   Outputs :: "output_function list"
-  Updates :: "update_function list"
+  Updates :: "update_functions"
 text_raw\<open>}%endsnip\<close>
 
 definition same_structure :: "transition \<Rightarrow> transition \<Rightarrow> bool" where
@@ -26,8 +31,11 @@ definition same_structure :: "transition \<Rightarrow> transition \<Rightarrow> 
     length (Outputs t1) = length (Outputs t2)
   )"
 
+definition finfun_as_list :: "('a::linorder \<Rightarrow>f 'b) \<Rightarrow> ('a \<times> 'b) list" where
+  "finfun_as_list f = map (\<lambda>x. (x, f $ x)) (finfun_to_list f)"
+
 definition enumerate_inputs :: "transition \<Rightarrow> nat set" where
-  "enumerate_inputs t = (\<Union> (set (map enumerate_gexp_inputs (Guard t)))) \<union>
+  "enumerate_inputs t = (\<Union> (set (map enumerate_gexp_inputs (Guards t)))) \<union>
                         (\<Union> (set (map enumerate_aexp_inputs (Outputs t)))) \<union>
                         (\<Union> (set (map (\<lambda>(_, u). enumerate_aexp_inputs u) (Updates t))))"
 
@@ -37,99 +45,26 @@ definition max_input :: "transition \<Rightarrow> nat option" where
 definition total_max_input :: "transition \<Rightarrow> nat" where
   "total_max_input t = (case max_input t of None \<Rightarrow> 0 | Some a \<Rightarrow> a)"
 
-definition enumerate_registers :: "transition \<Rightarrow> nat set" where
-  "enumerate_registers t = (\<Union> (set (map enumerate_gexp_regs (Guard t)))) \<union>
-                           (\<Union> (set (map enumerate_aexp_regs (Outputs t)))) \<union>
-                           (\<Union> (set (map (\<lambda>(_, u). enumerate_aexp_regs u) (Updates t)))) \<union>
-                           (\<Union> (set (map (\<lambda>(r, _). enumerate_aexp_regs (V (R r))) (Updates t))))"
-
-lemma gexp_regs_list: "\<exists>l. \<Union> (set (map enumerate_gexp_regs G)) = set l"
-proof(induct G)
-  case Nil
-  then show ?case
-    by simp
-next
-  case (Cons a G)
-  then show ?case
-    by (metis enumerate_gexp_regs_list Sup_insert list.simps(15) list.simps(9) set_append)
-qed
-
-lemma outputs_regs_list: "\<exists>l. \<Union> (set (map enumerate_aexp_regs P)) = set l"
-proof(induct P)
-  case Nil
-  then show ?case
-    by simp
-next
-  case (Cons a P)
-  then show ?case
-    by (metis enumerate_aexp_regs_list Sup_insert list.simps(15) list.simps(9) set_append)
-qed
-
-lemma updates_regs_list_1: "\<exists>l. \<Union> (set (map (\<lambda>(uu, y). enumerate_aexp_regs y) U)) = set l"
-proof(induct U)
-  case Nil
-  then show ?case
-    by simp
-next
-  case (Cons a U)
-  then show ?case
-    apply clarify
-    apply simp
-    apply (cases a)
-    apply simp
-    by (metis enumerate_aexp_regs_list set_append)
-qed
-
-lemma updates_regs_list_2: "\<exists>l. \<Union> (set (map (\<lambda>(r, uu). enumerate_aexp_regs (V (R r))) U)) = set l"
-proof(induct U)
-case Nil
-  then show ?case
-    by simp
-next
-  case (Cons a U)
-  then show ?case
-    apply clarify
-    apply simp
-    apply (cases a)
-    apply simp
-    by (metis List.set_insert)
-qed
-
-lemma enumerate_registers_list: "\<exists>l. enumerate_registers t = set l"
-  unfolding enumerate_registers_def
-  using gexp_regs_list[of "Guard t"]
-        outputs_regs_list[of "Outputs t"]
-        updates_regs_list_1[of "Updates t"]
-        updates_regs_list_2[of "Updates t"]
-  by (metis set_union)
+definition enumerate_regs :: "transition \<Rightarrow> nat set" where
+  "enumerate_regs t = (\<Union> (set (map GExp.enumerate_regs (Guards t)))) \<union>
+                      (\<Union> (set (map AExp.enumerate_regs (Outputs t)))) \<union>
+                      (\<Union> (set (map (\<lambda>(_, u). AExp.enumerate_regs u) (Updates t)))) \<union>
+                      (\<Union> (set (map (\<lambda>(r, _). AExp.enumerate_regs (V (R r))) (Updates t))))"
 
 definition max_reg :: "transition \<Rightarrow> nat option" where
-  "max_reg t = (if enumerate_registers t = {} then None else Some (Max (enumerate_registers t)))"
-
-lemma max_reg_none_no_updates: "Transition.max_reg t = None \<Longrightarrow> Updates t = []"
-  apply (simp add: Transition.max_reg_def)
-  apply (case_tac "enumerate_registers t = {}")
-   apply (simp add: enumerate_registers_def)
-   apply (case_tac "Updates t")
-  by auto
+  "max_reg t = (if enumerate_regs t = {} then None else Some (Max (enumerate_regs t)))"
 
 definition total_max_reg :: "transition \<Rightarrow> nat" where
   "total_max_reg t = (case max_reg t of None \<Rightarrow> 0 | Some a \<Rightarrow> a)"
 
+definition enumerate_ints :: "transition \<Rightarrow> int set" where
+  "enumerate_ints t = (\<Union> (set (map enumerate_gexp_ints (Guards t)))) \<union>
+                      (\<Union> (set (map enumerate_aexp_ints (Outputs t)))) \<union>
+                      (\<Union> (set (map (\<lambda>(_, u). enumerate_aexp_ints u) (Updates t)))) \<union>
+                      (\<Union> (set (map (\<lambda>(r, _). enumerate_aexp_ints (V (R r))) (Updates t))))"
+
 definition valid_transition :: "transition \<Rightarrow> bool" where
   "valid_transition t = (case max_input t of None \<Rightarrow> Arity t = 0 | Some x \<Rightarrow> x < Arity t)"
-
-definition enumerate_strings :: "transition \<Rightarrow> String.literal set" where
-  "enumerate_strings t = (\<Union> (set (map enumerate_gexp_strings (Guard t)))) \<union>
-                         (\<Union> (set (map enumerate_aexp_strings (Outputs t)))) \<union>
-                         (\<Union> (set (map (\<lambda>(_, u). enumerate_aexp_strings u) (Updates t)))) \<union>
-                         (\<Union> (set (map (\<lambda>(r, _). enumerate_aexp_strings (V (R r))) (Updates t))))"
-
-definition enumerate_ints :: "transition \<Rightarrow> int set" where
-  "enumerate_ints t = (\<Union> (set (map enumerate_gexp_ints (Guard t)))) \<union>
-                         (\<Union> (set (map enumerate_aexp_ints (Outputs t)))) \<union>
-                         (\<Union> (set (map (\<lambda>(_, u). enumerate_aexp_ints u) (Updates t)))) \<union>
-                         (\<Union> (set (map (\<lambda>(r, _). enumerate_aexp_ints (V (R r))) (Updates t))))"
 
 definition can_take :: "nat \<Rightarrow> vname gexp list \<Rightarrow> inputs \<Rightarrow> registers \<Rightarrow> bool" where
   "can_take a g i r = (length i = a \<and> apply_guards g (join_ir i r))"
@@ -137,18 +72,31 @@ definition can_take :: "nat \<Rightarrow> vname gexp list \<Rightarrow> inputs \
 lemma can_take_empty [simp]: "length i = a \<Longrightarrow> can_take a [] i c"
   by (simp add: can_take_def)
 
-lemma can_take_subset_append: "set (Guard t) \<subseteq> set (Guard t') \<Longrightarrow> can_take a (Guard t @ Guard t') i c = can_take a (Guard t') i c"
+lemma can_take_subset_append:
+  assumes "set (Guards t) \<subseteq> set (Guards t')"
+  shows "can_take a (Guards t @ Guards t') i c = can_take a (Guards t') i c"
+  using assms
   by (simp add: apply_guards_subset_append can_take_def)
 
-definition "can_take_transition t i r = can_take (Arity t) (Guard t) i r"
+definition "can_take_transition t i r = can_take (Arity t) (Guards t) i r"
 
-lemma can_take_transition_empty_guard: "Guard t = [] \<Longrightarrow> \<exists>i. can_take_transition t i c"
+lemma can_take_transition_empty_guard: "Guards t = [] \<Longrightarrow> \<exists>i. can_take_transition t i c"
   by (simp add: can_take_transition_def can_take_def Ex_list_of_length)
 
-lemma valid_list_can_take: "\<forall>g \<in> set (Guard t). valid g \<Longrightarrow> \<exists>i. can_take_transition t i c"
+lemma valid_list_can_take: "\<forall>g \<in> set (Guards t). valid g \<Longrightarrow> \<exists>i. can_take_transition t i c"
   by (simp add: can_take_transition_def can_take_def apply_guards_def valid_def Ex_list_of_length)
 
-lemma cant_take_if: "\<exists>g \<in> set (Guard t). gval g (join_ir i r) \<noteq> true \<Longrightarrow> \<not> can_take_transition t i r"
+lemma cant_take_if:
+  "\<exists>g \<in> set (Guards t). gval g (join_ir i r) \<noteq> true \<Longrightarrow> \<not> can_take_transition t i r"
   using apply_guards_cons apply_guards_rearrange can_take_def can_take_transition_def by blast
+
+inductive eq_upto_rename :: "transition \<Rightarrow> transition \<Rightarrow> bool" where
+  "Label t1 = Label t2 \<Longrightarrow>
+   Arity t1 = Arity t2 \<Longrightarrow>
+   bij f \<Longrightarrow>
+   image (\<lambda>g1. GExp.rename_regs g1 f) (set g1) = set g2 \<Longrightarrow>
+   map (\<lambda>p. AExp.rename_regs p f) o1 = o2 \<Longrightarrow>
+   map_of (map (\<lambda>(r, u). (f r, AExp.rename_regs u f)) (Updates t1)) = map_of (Updates t2) \<Longrightarrow>
+  eq_upto_rename t1 t2"
 
 end
