Value.thy
@@ -2,6 +2,12 @@ theory Value
 imports Trilean
 begin
 
+section\<open>Values\<close>
+
+text\<open>Our EFSM implementation can currently handle integers and strings. Here we define a sum type
+which combines these. We also define an arithmetic in terms of values such that EFSMs do not need
+to be strongly typed.\<close>
+
 text_raw\<open>\snip{valuetype}{1}{2}{%\<close>
 datatype "value" = Num int | Str String.literal
 text_raw\<open>}%endsnip\<close>
@@ -14,16 +20,20 @@ fun MaybeArithInt :: "(int \<Rightarrow> int \<Rightarrow> int) \<Rightarrow> va
   "MaybeArithInt f (Some (Num x)) (Some (Num y)) = Some (Num (f x y))" |
   "MaybeArithInt _ _ _ = None"
 
-lemma MaybeArithInt_not_None: "MaybeArithInt f a b \<noteq> None = (\<exists>n n'. a = Some (Num n) \<and> b = Some (Num n'))"
+lemma MaybeArithInt_not_None:
+  "MaybeArithInt f a b \<noteq> None = (\<exists>n n'. a = Some (Num n) \<and> b = Some (Num n'))"
   using MaybeArithInt.elims MaybeArithInt.simps(1) by blast
 
-lemma MaybeArithInt_Some: "MaybeArithInt f a b = Some (Num x) = (\<exists>n n'. a = Some (Num n) \<and> b = Some (Num n') \<and> f n n' = x)"
+lemma MaybeArithInt_Some:
+  "MaybeArithInt f a b = Some (Num x) = (\<exists>n n'. a = Some (Num n) \<and> b = Some (Num n') \<and> f n n' = x)"
   using MaybeArithInt.elims MaybeArithInt.simps(1) by blast
 
-lemma MaybeArithInt_None: "(MaybeArithInt f a1 a2 = None) = (\<nexists>n n'. a1 = Some (Num n) \<and> a2 = Some (Num n'))"
+lemma MaybeArithInt_None:
+  "(MaybeArithInt f a1 a2 = None) = (\<nexists>n n'. a1 = Some (Num n) \<and> a2 = Some (Num n'))"
   using MaybeArithInt_not_None by blast
 
-lemma MaybeArithInt_Not_Num: "(\<forall>n. MaybeArithInt f a1 a2 \<noteq> Some (Num n)) = (MaybeArithInt f a1 a2 = None)"
+lemma MaybeArithInt_Not_Num:
+  "(\<forall>n. MaybeArithInt f a1 a2 \<noteq> Some (Num n)) = (MaybeArithInt f a1 a2 = None)"
   by (metis MaybeArithInt.elims option.distinct(1))
 
 lemma MaybeArithInt_never_string: "MaybeArithInt f a b \<noteq> Some (Str x)"
@@ -40,130 +50,27 @@ lemma value_plus_symmetry: "value_plus x y = value_plus y x"
 
 definition "value_minus = MaybeArithInt (-)"
 
-lemma minus_never_string: "value_minus a b \<noteq> Some (Str x)"
+lemma value_minus_never_string: "value_minus a b \<noteq> Some (Str x)"
   by (simp add: MaybeArithInt_never_string value_minus_def)
 
 definition "value_times = MaybeArithInt (*)"
+
+lemma value_times_never_string: "value_times a b \<noteq> Some (Str x)"
+  by (simp add: MaybeArithInt_never_string value_times_def)
 
 fun MaybeBoolInt :: "(int \<Rightarrow> int \<Rightarrow> bool) \<Rightarrow> value option \<Rightarrow> value option \<Rightarrow> trilean" where
   "MaybeBoolInt f (Some (Num a)) (Some (Num b)) = (if f a b then true else false)" |
   "MaybeBoolInt _ _ _ = invalid"
 
-lemma MaybeBoolInt_lt: "MaybeBoolInt (\<lambda>x y. y < x) (Some (Num n')) r = false \<Longrightarrow> \<exists>n. r = Some (Num n) \<and> n' \<le> n"
-proof(induct n')
-  case (nonneg n)
-  then show ?case
-    using MaybeBoolInt.elims by force
-next
-  case (neg n)
-  then show ?case
-    using MaybeBoolInt.elims by force
-qed
-
-lemma MaybeBoolInt_not_num_1: "\<forall>n. r \<noteq> Some (Num n) \<Longrightarrow> MaybeBoolInt f n r = invalid"
-  apply (cases r)
-   apply simp
-  apply (case_tac a)
-  by auto
+lemma MaybeBoolInt_not_num_1:
+  "\<forall>n. r \<noteq> Some (Num n) \<Longrightarrow> MaybeBoolInt f n r = invalid"
+  using MaybeBoolInt.elims by blast
 
 definition value_gt :: "value option \<Rightarrow> value option \<Rightarrow> trilean"  where
-  "value_gt a b \<equiv> MaybeBoolInt (\<lambda>x::int.\<lambda>y::int.(x>y)) a b"
+  "value_gt a b \<equiv> MaybeBoolInt (>) a b"
 
 definition value_eq :: "value option \<Rightarrow> value option \<Rightarrow> trilean"  where
   "value_eq a b \<equiv> (if a = b then true else false)"
 declare value_eq_def [simp]
-
-instantiation "value" :: linorder begin
-fun less_eq_value :: "value \<Rightarrow> value \<Rightarrow> bool" where
-  "less_eq_value (Num n) (Str s) = True" |
-  "less_eq_value (Str s) (Num n) = False" |
-  "less_eq_value (Str n) (Str s) = less_eq n s" |
-  "less_eq_value (Num n) (Num s) = less_eq n s"
-
-fun less_value :: "value \<Rightarrow> value \<Rightarrow> bool" where
-  "less_value (Num n) (Str s) = True" |
-  "less_value (Str s) (Num n) = False" |
-  "less_value (Str n) (Str s) = less n s" |
-  "less_value (Num n) (Num s) = less n s"
-
-instance proof
-  fix x y::"value"
-  show "(x < y) = (x \<le> y \<and> \<not> y \<le> x)"
-  proof (induct x)
-    case (Num x)
-    then show ?case
-      apply (cases y)
-      by auto
-  next
-    case (Str x)
-    then show ?case
-      apply (cases y)
-      by auto
-  qed
-  fix x :: "value"
-  show "x \<le> x"
-    apply (cases x)
-    by auto
-  fix x y z::"value"
-  show "x \<le> y \<Longrightarrow> y \<le> z \<Longrightarrow> x \<le> z"
-  proof (induct x)
-    case (Num n)
-    then show ?case
-    proof (induct y)
-      case (Num x)
-      then show ?case
-        apply (cases z)
-        by auto
-    next
-      case (Str x)
-      then show ?case
-        apply (cases z)
-        by auto
-    qed
-  next
-    case (Str s)
-    then show ?case
-    proof (induct y)
-      case (Num x)
-      then show ?case
-        apply (cases z)
-        by auto
-    next
-      case (Str x)
-      then show ?case
-        apply (cases z)
-        by auto
-    qed
-  qed
-next
-  fix x y :: "value"
-  show "x \<le> y \<Longrightarrow> y \<le> x \<Longrightarrow> x = y"
-  proof (induct x)
-    case (Num x)
-    then show ?case
-      apply (cases y)
-      by auto
-  next
-    case (Str x)
-    then show ?case
-      apply (cases y)
-      by auto
-  qed
-next
-  fix x y::"value"
-  show "x \<le> y \<or> y \<le> x"
-  proof (induct x)
-    case (Num x)
-    then show ?case
-      apply (cases y)
-      by auto
-  next
-    case (Str x)
-    then show ?case
-      apply (cases y)
-      by auto
-  qed
-qed
-end
 
 end
