examples/Drinks_Machine.thy
@@ -21,7 +21,7 @@ definition select :: "transition" where
 "select \<equiv> \<lparr>
         Label = STR ''select'',
         Arity = 1,
-        Guard = [], \<comment> \<open> No guards \<close>
+        Guards = [], \<comment> \<open> No guards \<close>
         Outputs = [],
         Updates = [ \<comment> \<open> Two updates: \<close>
                     (1, V (I 0)), \<comment> \<open>  Firstly set value of r1 to value of i1 \<close>
@@ -34,7 +34,7 @@ definition coin :: "transition" where
 "coin \<equiv> \<lparr>
         Label = STR ''coin'',
         Arity = 1,
-        Guard = [],
+        Guards = [],
         Outputs = [Plus (V (R 2)) (V (I 0))],
         Updates = [
                     (1, V (R 1)),
@@ -47,7 +47,7 @@ definition vend :: "transition" where
 "vend \<equiv> \<lparr>
         Label = STR ''vend'',
         Arity = 0,
-        Guard = [(Ge (V (R 2)) (L (Num 100)))],
+        Guards = [(Ge (V (R 2)) (L (Num 100)))],
         Outputs =  [(V (R 1))],
         Updates = [(1, V (R 1)), (2, V (R 2))]
       \<rparr>"
@@ -56,7 +56,7 @@ definition vend_fail :: "transition" where
 "vend_fail \<equiv> \<lparr>
         Label = STR ''vend'',
         Arity = 0,
-        Guard = [(Lt (V (R 2)) (L (Num 100)))],
+        Guards = [(Lt (V (R 2)) (L (Num 100)))],
         Outputs =  [],
         Updates = [(1, V (R 1)), (2, V (R 2))]
       \<rparr>"
@@ -75,7 +75,8 @@ lemma "S drinks = {|0, 1, 2|}"
   apply (simp add: S_def drinks_def)
   by auto
 
-lemma possible_steps_0:  "length i = 1 \<Longrightarrow> possible_steps drinks 0 r (STR ''select'') i = {|(1, select)|}"
+lemma possible_steps_0:
+ "length i = 1 \<Longrightarrow> possible_steps drinks 0 r (STR ''select'') i = {|(1, select)|}"
   apply (simp add: possible_steps_singleton drinks_def)
   apply safe
   by (simp_all add: transitions apply_guards_def)
@@ -86,42 +87,50 @@ lemma first_step_select:
   apply safe
   by (simp_all add: transitions)
 
-lemma drinks_vend_insufficient: "r $ 2 = Some (Num x1) \<Longrightarrow> x1 < 100 \<Longrightarrow> possible_steps drinks 1 r (STR ''vend'') [] = {|(1, vend_fail)|}"
+lemma drinks_vend_insufficient:
+"r $ 2 = Some (Num x1) \<Longrightarrow> x1 < 100 \<Longrightarrow> possible_steps drinks 1 r (STR ''vend'') [] = {|(1, vend_fail)|}"
   apply (simp add: possible_steps_singleton drinks_def)
   apply safe
   by (simp_all add: transitions apply_guards_def value_gt_def join_ir_def connectives)
 
-lemma drinks_vend_invalid: "\<nexists>n. r $ 2 = Some (Num n) \<Longrightarrow> possible_steps drinks 1 r (STR ''vend'') [] = {||}"
+lemma drinks_vend_invalid:
+"\<nexists>n. r $ 2 = Some (Num n) \<Longrightarrow> possible_steps drinks 1 r (STR ''vend'') [] = {||}"
   apply (simp add: possible_steps_empty drinks_def can_take_transition_def can_take_def transitions)
   by (simp add: MaybeBoolInt_not_num_1 value_gt_def)
 
-lemma possible_steps_1_coin: "length i = 1 \<Longrightarrow> possible_steps drinks 1 r (STR ''coin'') i = {|(1, coin)|}"
+lemma possible_steps_1_coin:
+"length i = 1 \<Longrightarrow> possible_steps drinks 1 r (STR ''coin'') i = {|(1, coin)|}"
   apply (simp add: possible_steps_singleton drinks_def)
   apply safe
   by (simp_all add: transitions)
 
-lemma possible_steps_2_vend: "\<exists>n. r $ 2 = Some (Num n) \<and> n \<ge> 100 \<Longrightarrow> possible_steps drinks 1 r (STR ''vend'') [] = {|(2, vend)|}"
+lemma possible_steps_2_vend:
+"\<exists>n. r $ 2 = Some (Num n) \<and> n \<ge> 100 \<Longrightarrow> possible_steps drinks 1 r (STR ''vend'') [] = {|(2, vend)|}"
   apply (simp add: possible_steps_singleton drinks_def)
   apply safe
   by (simp_all add: transitions apply_guards_def value_gt_def join_ir_def connectives)
 
-lemma accepts_from_2: "accepts drinks 1 (<>(1 := d, 2 := Num 100)) [(STR ''vend'', [])]"
+lemma accepts_from_2:
+"accepts drinks 1 (<>(1 := d, 2 := Num 100)) [(STR ''vend'', [])]"
   apply (rule accepts.step[of 2 vend])
    apply (simp add: possible_steps_2_vend)
   by (simp add: accepts.base)
 
-lemma accepts_from_1a: "accepts drinks 1 (<>(1 := d, 2 := Num 50)) [(STR ''coin'', [Num 50]), (STR ''vend'', [])]"
+lemma accepts_from_1a:
+"accepts drinks 1 (<>(1 := d, 2 := Num 50)) [(STR ''coin'', [Num 50]), (STR ''vend'', [])]"
   apply (rule accepts.step[of 1 coin])
    apply (simp add: possible_steps_1_coin)
   by (simp add: coin_def join_ir_def input2state_def value_plus_def finfun_update_twist accepts_from_2)
 
-lemma accepts_from_1: "accepts drinks 1 (<>(2 := Num 0, 1 := d))
+lemma accepts_from_1:
+"accepts drinks 1 (<>(2 := Num 0, 1 := d))
      [(STR ''coin'', [Num 50]), (STR ''coin'', [Num 50]), (STR ''vend'', [])]"
   apply (rule accepts.step[of 1 coin])
    apply (simp add: possible_steps_1_coin)
   by (simp add: coin_def join_ir_def input2state_def value_plus_def finfun_update_twist accepts_from_1a)
 
-lemma purchase_coke: "observe_trace drinks 0 <> [(STR ''select'', [Str ''coke'']), (STR ''coin'', [Num 50]), (STR ''coin'', [Num 50]), (STR ''vend'', [])] =
+lemma purchase_coke:
+"observe_trace drinks 0 <> [(STR ''select'', [Str ''coke'']), (STR ''coin'', [Num 50]), (STR ''coin'', [Num 50]), (STR ''vend'', [])] =
                        [[], [Some (Num 50)], [Some (Num 100)], [Some (Str ''coke'')]]"
   apply (rule observe_trace_possible_step)
      apply (simp add: possible_steps_0)
@@ -144,7 +153,8 @@ lemma purchase_coke: "observe_trace drinks 0 <> [(STR ''select'', [Str ''coke'']
    apply simp
   by simp
 
-lemma rejects_input: "l \<noteq> STR ''coin'' \<Longrightarrow> l \<noteq> STR ''vend'' \<Longrightarrow> \<not> accepts drinks 1 d' [(l, i)]"
+lemma rejects_input:
+"l \<noteq> STR ''coin'' \<Longrightarrow> l \<noteq> STR ''vend'' \<Longrightarrow> \<not> accepts drinks 1 d' [(l, i)]"
   apply (rule no_possible_steps_rejects)
   by (simp add: possible_steps_empty drinks_def can_take_transition_def can_take_def transitions)
 
@@ -156,51 +166,61 @@ lemma rejects_accepts_prefix:
   apply (simp add: possible_steps_0 select_def join_ir_def input2state_def)
   using rejects_input by blast
 
-lemma rejects_termination: "observe_trace drinks 0 <> [(STR ''select'', [Str ''coke'']), (STR ''rejects'', [Num 50]), (STR ''coin'', [Num 50])] = [[]]"
+lemma rejects_termination:
+"observe_trace drinks 0 <> [(STR ''select'', [Str ''coke'']), (STR ''rejects'', [Num 50]), (STR ''coin'', [Num 50])] = [[]]"
   apply (rule observe_trace_step)
    apply (simp add: step_def possible_steps_0 select_def)
   apply (rule observe_trace_no_possible_step)
   by (simp add: possible_steps_empty drinks_def can_take_transition_def can_take_def transitions)
 
 (* Part of Example 2 in Foster et. al. *)
-lemma r2_0_vend: "can_take_transition vend i r \<Longrightarrow> \<exists>n. r $ 2 = Some (Num n) \<and> n \<ge> 100" (* You can't take vend immediately after taking select *)
-  apply (simp add: can_take_transition_def can_take_def vend_def apply_guards_def maybe_negate_true maybe_or_false connectives)
-  by (simp add: value_gt_def join_ir_def MaybeBoolInt_lt)
+lemma r2_0_vend:
+"can_take_transition vend i r \<Longrightarrow> \<exists>n. r $ 2 = Some (Num n) \<and> n \<ge> 100" (* You can't take vend immediately after taking select *)
+  apply (simp add: can_take_transition_def can_take_def vend_def apply_guards_def maybe_negate_true maybe_or_false connectives value_gt_def)
+  using MaybeBoolInt.elims by force
 
-lemma drinks_vend_sufficient: "r $ 2 = Some (Num x1) \<Longrightarrow>
+lemma drinks_vend_sufficient:
+"r $ 2 = Some (Num x1) \<Longrightarrow>
                 x1 \<ge> 100 \<Longrightarrow>
                 possible_steps drinks 1 r (STR ''vend'') [] = {|(2, vend)|}"
   using possible_steps_2_vend by blast
 
-lemma drinks_end: "possible_steps drinks 2 r a b = {||}"
+lemma drinks_end:
+"possible_steps drinks 2 r a b = {||}"
   apply (simp add: possible_steps_def drinks_def transitions)
   by force
 
-lemma drinks_vend_r2_String: "r $ 2 = Some (value.Str x2) \<Longrightarrow> possible_steps drinks 1 r (STR ''vend'') [] = {||}"
+lemma drinks_vend_r2_String:
+"r $ 2 = Some (value.Str x2) \<Longrightarrow> possible_steps drinks 1 r (STR ''vend'') [] = {||}"
   apply (simp add: possible_steps_empty drinks_def can_take_transition_def can_take_def transitions)
   by (simp add: value_gt_def)
 
-lemma drinks_vend_r2_rejects: "\<nexists>n. r $ 2 = Some (Num n) \<Longrightarrow> step drinks 1 r (STR ''vend'') [] = None"
+lemma drinks_vend_r2_rejects:
+"\<nexists>n. r $ 2 = Some (Num n) \<Longrightarrow> step drinks 1 r (STR ''vend'') [] = None"
   apply (rule no_possible_steps_1)
   apply (simp add: possible_steps_empty drinks_def can_take_transition_def can_take_def transitions)
   by (simp add: MaybeBoolInt_not_num_1 value_gt_def)
 
-lemma drinks_0_rejects: "\<not> (fst a = STR ''select'' \<and> length (snd a) = 1) \<Longrightarrow>
+lemma drinks_0_rejects:
+"\<not> (fst a = STR ''select'' \<and> length (snd a) = 1) \<Longrightarrow>
     (possible_steps drinks 0 r (fst a) (snd a)) = {||}"
   apply (simp add: drinks_def possible_steps_def transitions)
   by force
 
-lemma drinks_vend_empty: "(possible_steps drinks 0 <> (STR ''vend'') []) = {||}"
+lemma drinks_vend_empty:
+"(possible_steps drinks 0 <> (STR ''vend'') []) = {||}"
   using drinks_0_rejects
   by auto
 
-lemma drinks_1_rejects: "fst a = STR ''coin'' \<longrightarrow> length (snd a) \<noteq> 1 \<Longrightarrow>
+lemma drinks_1_rejects:
+"fst a = STR ''coin'' \<longrightarrow> length (snd a) \<noteq> 1 \<Longrightarrow>
           a \<noteq> (STR ''vend'', []) \<Longrightarrow>
           possible_steps drinks 1 r (fst a) (snd a) = {||}"
   apply (simp add: possible_steps_empty drinks_def can_take_transition_def can_take_def transitions)
   by (metis decompose_pair)
 
-lemma drinks_rejects_future: "rejects drinks 2 d ((l, i)#t)"
+lemma drinks_rejects_future:
+"rejects drinks 2 d ((l, i)#t)"
   apply (rule no_possible_steps_rejects)
   by (simp add: possible_steps_empty drinks_def)
 
@@ -218,15 +238,18 @@ proof-
     using not_coin by auto
 qed
 
-lemma rejects_state_step: "s > 1 \<Longrightarrow> step drinks s r l i = None"
+lemma rejects_state_step:
+"s > 1 \<Longrightarrow> step drinks s r l i = None"
   apply (rule no_possible_steps_1)
   by (simp add: possible_steps_empty drinks_def)
 
-lemma invalid_other_states: "s > 1 \<Longrightarrow> rejects drinks s r ((aa, b) # t)"
+lemma invalid_other_states:
+"s > 1 \<Longrightarrow> rejects drinks s r ((aa, b) # t)"
   apply (rule no_possible_steps_rejects)
   by (simp add: possible_steps_empty drinks_def)
 
-lemma vend_ge_100: "possible_steps drinks 1 r l i = {|(2, vend)|} \<Longrightarrow> \<not>\<^sub>? value_gt (Some (Num 100)) (r $ 2) = trilean.true"
+lemma vend_ge_100:
+"possible_steps drinks 1 r l i = {|(2, vend)|} \<Longrightarrow> \<not>\<^sub>? value_gt (Some (Num 100)) (r $ 2) = trilean.true"
   apply (insert possible_steps_apply_guards[of drinks 1 r l i 2 vend])
   by (simp add: possible_steps_def apply_guards_def vend_def)
 
