FSet_Utils.thy
@@ -24,47 +24,10 @@ translations
   "\<nexists>x|\<in>|A. P" \<rightleftharpoons> "CONST fBall A (\<lambda>x. \<not>P)"
   "\<exists>!x|\<in>|A. P" \<rightharpoonup> "\<exists>!x. x |\<in>| A \<and> P"
 
-context includes fset.lifting begin
-  lift_definition fprod  :: "'a fset \<Rightarrow> 'b fset \<Rightarrow> ('a \<times> 'b) fset " (infixr "|\<times>|" 80) is "\<lambda>a b. fset a \<times> fset b"
-    by simp
-  
-  lift_definition fis_singleton :: "'a fset \<Rightarrow> bool" is "\<lambda>A. is_singleton (fset A)".
-end
-
-lemma fprod_empty_l: "{||} |\<times>| a = {||}"
-  using bot_fset_def fprod.abs_eq by force
-
-lemma fprod_empty_r: "a |\<times>| {||} = {||}"
-  by (simp add: fprod_def bot_fset_def Abs_fset_inverse)
-
-lemmas fprod_empty = fprod_empty_l fprod_empty_r
-
-lemma fprod_finsert: "(finsert a as) |\<times>| (finsert b bs) = finsert (a, b) (fimage (\<lambda>b. (a, b)) bs |\<union>| fimage (\<lambda>a. (a, b)) as |\<union>| (as |\<times>| bs))"
-  apply (simp add: finsert_def fprod_def Abs_fset_inverse)
-  apply (rule arg_cong[of "(insert (a, b) (fset as \<times> insert b (fset bs) \<union> insert a (fset as) \<times> fset bs))"
-                    "(insert (a, b) (Pair a ` fset bs \<union> (\<lambda>a. (a, b)) ` fset as \<union> fset as \<times> fset bs))"
-                    Abs_fset])
-  by auto
-
-lemma fprod_member: "x |\<in>| xs \<Longrightarrow> y |\<in>| ys \<Longrightarrow> (x, y) |\<in>| xs |\<times>| ys"
-  by (simp add: fmember_def fprod_def Abs_fset_inverse)
-
-lemma fprod_subseteq: "x |\<subseteq>| x' \<and> y |\<subseteq>| y' \<Longrightarrow> x |\<times>| y |\<subseteq>| x' |\<times>| y'"
-  apply (simp add: fprod_def less_eq_fset_def Abs_fset_inverse)
-  by auto
-
-lemma fimage_fprod: "(a, b) |\<in>| A |\<times>| B \<Longrightarrow> f a b |\<in>| (\<lambda>(x, y). f x y) |`| (A |\<times>| B)"
-  by force
-
-lemma fprod_singletons: "{|a|} |\<times>| {|b|} = {|(a, b)|}"
-  apply (simp add: fprod_def)
-  by (metis fset_inverse fset_simps(1) fset_simps(2))
-
-lemma fprod_equiv: "(fset (f |\<times>| f') = s) = (((fset f) \<times> (fset f')) = s)"
-  by (simp add: fprod_def Abs_fset_inverse)
-
-lemma fis_singleton_alt: "fis_singleton f = (\<exists>e. f = {|e|})"
-  by (metis fis_singleton.rep_eq fset_inverse fset_simps(1) fset_simps(2) is_singleton_def)
+lemma fset_of_list_remdups [simp]: "fset_of_list (remdups l) = fset_of_list l"
+  apply (induct l)
+   apply simp
+  by (simp add: finsert_absorb fset_of_list_elem)
 
 definition "fSum \<equiv> fsum (\<lambda>x. x)"
 
@@ -75,23 +38,16 @@ lemma Abs_ffilter: "(ffilter f s = s') = ({e \<in> (fset s). f e} = (fset s'))"
   by (simp add: ffilter_def fset_both_sides Abs_fset_inverse Set.filter_def)
 
 lemma ffilter_empty [simp]: "ffilter f {||} = {||}"
-  apply (simp add: ffilter_def fset_both_sides Abs_fset_inverse)
   by auto
 
-lemma ffilter_finsert: "ffilter f (finsert a s) = (if f a then finsert a (ffilter f s) else (ffilter f s))"
+lemma ffilter_finsert:
+  "ffilter f (finsert a s) = (if f a then finsert a (ffilter f s) else (ffilter f s))"
   apply simp
   apply standard
    apply (simp add: ffilter_def fset_both_sides Abs_fset_inverse)
    apply auto[1]
   apply (simp add: ffilter_def fset_both_sides Abs_fset_inverse)
   by auto
-
-lemma singleton_singleton [simp]: "fis_singleton {|a|}"
-  by (simp add: fis_singleton_def)
-
-lemma not_singleton_empty [simp]: "\<not> fis_singleton {||}"
-  apply (simp add: fis_singleton_def)
-  by (simp add: is_singleton_altdef)
 
 lemma fset_equiv: "(f1 = f2) = (fset f1 = fset f2)"
   by (simp add: fset_inject)
@@ -102,24 +58,14 @@ lemma finsert_equiv: "(finsert e f = f') = (insert e (fset f) = (fset f'))"
 lemma filter_elements: "x |\<in>| Abs_fset (Set.filter f (fset s)) = (x \<in> (Set.filter f (fset s)))"
   by (metis ffilter.rep_eq fset_inverse notin_fset)
 
-lemma singleton_equiv: "is_singleton s \<Longrightarrow> (the_elem s = i) = (s = {i})"
-  by (meson is_singleton_the_elem the_elem_eq)
-
-lemma sorted_list_of_empty [simp]: "sorted_list_of_fset {||} = []"
+lemma sorted_list_of_fempty [simp]: "sorted_list_of_fset {||} = []"
   by (simp add: sorted_list_of_fset_def)
 
 lemma fmember_implies_member: "e |\<in>| f \<Longrightarrow> e \<in> fset f"
   by (simp add: fmember_def)
 
 lemma fold_union_ffUnion: "fold (|\<union>|) l {||} = ffUnion (fset_of_list l)"
-proof(induct l rule: rev_induct)
-case Nil
-  then show ?case by simp
-next
-  case (snoc a l)
-  then show ?case
-    by simp
-qed
+by(induct l rule: rev_induct, auto)
 
 lemma filter_filter: "ffilter P (ffilter Q xs) = ffilter (\<lambda>x. Q x \<and> P x) xs"
   by auto
@@ -130,16 +76,16 @@ lemma fsubset_strict: "x2 |\<subset>| x1 \<Longrightarrow> \<exists>e. e |\<in>|
 lemma fsubset: "x2 |\<subset>| x1 \<Longrightarrow> \<nexists>e. e |\<in>| x2 \<and> e |\<notin>| x1"
   by auto
 
-lemma size_fsubset_elem: 
-  "\<exists>e. e |\<in>| x1 \<and> e |\<notin>| x2 \<Longrightarrow>
-   \<nexists>e. e |\<in>| x2 \<and> e |\<notin>| x1 \<Longrightarrow>
-   size x2 < size x1"
+lemma size_fsubset_elem:
+  assumes "\<exists>e. e |\<in>| x1 \<and> e |\<notin>| x2"
+      and "\<nexists>e. e |\<in>| x2 \<and> e |\<notin>| x1"
+    shows "size x2 < size x1"
+  using assms
   apply (simp add: fmember_def)
   by (metis card_seteq finite_fset linorder_not_le subsetI)
 
 lemma size_fsubset: "x2 |\<subset>| x1 \<Longrightarrow> size x2 < size x1"
-  using fsubset fsubset_strict size_fsubset_elem
-  by metis
+  by (metis fsubset fsubset_strict size_fsubset_elem)
 
 definition fremove :: "'a \<Rightarrow> 'a fset \<Rightarrow> 'a fset"
   where [code_abbrev]: "fremove x A = A - {|x|}"
@@ -151,29 +97,11 @@ lemma ffilter_singleton: "f e \<Longrightarrow> ffilter f {|e|} = {|e|}"
   apply (simp add: ffilter_def fset_both_sides Abs_fset_inverse)
   by auto
 
-lemma ffilter_true: "ffilter (\<lambda>x. True) f = f"
-  apply (simp add: ffilter_def fset_both_sides Abs_fset_inverse)
-  by auto
-
-lemma ffilter_true_pair: "ffilter (\<lambda>(x, y). True) f = f"
-  apply (simp add: ffilter_def fset_both_sides Abs_fset_inverse)
-  by auto
-
-lemma ffilter_out_all: "\<forall>e |\<in>| f. \<not>P e \<Longrightarrow> ffilter P f = {||}"
-  apply (simp add: ffilter_def fBall_def fset_both_sides Abs_fset_inverse)
-  by auto
-
 lemma fset_eq_alt: "(x = y) = (x |\<subseteq>| y \<and> size x = size y)"
   by (metis exists_least_iff le_less size_fsubset)
 
-definition fimages :: "('a \<Rightarrow> 'b fset) \<Rightarrow> 'a fset \<Rightarrow> 'b fset" where
-  "fimages f xs = ffUnion (fimage f xs)"
-
 lemma ffold_empty [simp]: "ffold f b {||} = b"
   by (simp add: ffold_def)
-
-lemma exists_fset_of_list: "\<exists>l. f = fset_of_list l"
-  using exists_fset_of_list by fastforce
 
 lemma sorted_list_of_fset_sort: "sorted_list_of_fset (fset_of_list l) = sort (remdups l)"
   by (simp add: fset_of_list.rep_eq sorted_list_of_fset.rep_eq sorted_list_of_set_sort_remdups)
@@ -190,6 +118,9 @@ lemma hd_sort_Min: "l \<noteq> [] \<Longrightarrow> hd (sort l) = Min (set l)"
 lemma hd_sort_remdups: "hd (sort (remdups l)) = hd (sort l)"
   by (metis hd_sort_Min remdups_eq_nil_iff set_remdups)
 
+lemma exists_fset_of_list: "\<exists>l. f = fset_of_list l"
+  using exists_fset_of_list by fastforce
+
 lemma hd_sorted_list_of_fset: "s \<noteq> {||} \<Longrightarrow> hd (sorted_list_of_fset s) = (fMin s)"
   apply (insert exists_fset_of_list[of s])
   apply (erule exE)
@@ -200,8 +131,7 @@ lemma hd_sorted_list_of_fset: "s \<noteq> {||} \<Longrightarrow> hd (sorted_list
 lemma fminus_filter_singleton: "fset_of_list l |-| {|x|} = fset_of_list (filter (\<lambda>e. e \<noteq> x) l)"
   by auto
 
-lemma card_minus_fMin: "s \<noteq> {||} \<Longrightarrow>
-       card (fset s - {fMin s}) < card (fset s)"
+lemma card_minus_fMin: "s \<noteq> {||} \<Longrightarrow> card (fset s - {fMin s}) < card (fset s)"
   by (metis Min_in bot_fset.rep_eq card_Diff1_less fMin.F.rep_eq finite_fset fset_equiv)
 
 (* Provides a deterministic way to fold fsets similar to List.fold that works with the code generator *)
@@ -238,7 +168,7 @@ lemma exists_sorted_distinct_fset_of_list: "\<exists>l. sorted l \<and> distinct
 lemma fset_of_list_empty [simp]: "(fset_of_list l = {||}) = (l = [])"
   by (metis fset_of_list.rep_eq fset_of_list_simps(1) set_empty)
 
-lemma ffold_ord_cons: 
+lemma ffold_ord_cons:
   assumes sorted: "sorted (h#t)"
     and distinct: "distinct (h#t)"
   shows "ffold_ord f (fset_of_list (h#t)) b = ffold_ord f (fset_of_list t) (f h b)"
@@ -252,18 +182,66 @@ proof-
     by (metis h_is_min remove_min fset_of_list_empty list.distinct(1))
 qed
 
-lemma sorted_distinct_ffold_ord: "sorted l \<Longrightarrow> distinct l \<Longrightarrow> ffold_ord f (fset_of_list l) b = fold f l b"
-proof(induct l arbitrary: b)
-case Nil
-  then show ?case
-    by simp
-next
-  case (Cons a l)
-  then show ?case
-    by (metis distinct.simps(2) ffold_ord_cons fold_simps(2) sorted.simps(2))
-qed
+lemma sorted_distinct_ffold_ord:
+  assumes "sorted l"
+      and "distinct l"
+    shows "ffold_ord f (fset_of_list l) b = fold f l b"
+  using assms
+  apply (induct l arbitrary: b)
+   apply simp
+  by (metis distinct.simps(2) ffold_ord_cons fold_simps(2) sorted.simps(2))
 
 lemma ffold_ord_fold_sorted: "ffold_ord f s b = fold f (sorted_list_of_fset s) b"
   by (metis exists_sorted_distinct_fset_of_list sorted_distinct_ffold_ord distinct_remdups_id sorted_list_of_fset_sort sorted_sort_id)
 
+context includes fset.lifting begin
+  lift_definition fprod  :: "'a fset \<Rightarrow> 'b fset \<Rightarrow> ('a \<times> 'b) fset " (infixr "|\<times>|" 80) is "\<lambda>a b. fset a \<times> fset b"
+    by simp
+  
+  lift_definition fis_singleton :: "'a fset \<Rightarrow> bool" is "\<lambda>A. is_singleton (fset A)".
+end
+
+lemma fprod_empty_l: "{||} |\<times>| a = {||}"
+  using bot_fset_def fprod.abs_eq by force
+
+lemma fprod_empty_r: "a |\<times>| {||} = {||}"
+  by (simp add: fprod_def bot_fset_def Abs_fset_inverse)
+
+lemmas fprod_empty = fprod_empty_l fprod_empty_r
+
+lemma fprod_finsert:
+  "(finsert a as) |\<times>| (finsert b bs) =
+   finsert (a, b) (fimage (\<lambda>b. (a, b)) bs |\<union>| fimage (\<lambda>a. (a, b)) as |\<union>| (as |\<times>| bs))"
+  apply (simp add: fprod_def fset_both_sides Abs_fset_inverse)
+  by auto
+
+lemma fprod_member: "x |\<in>| xs \<Longrightarrow> y |\<in>| ys \<Longrightarrow> (x, y) |\<in>| xs |\<times>| ys"
+  by (simp add: fmember_def fprod_def Abs_fset_inverse)
+
+lemma fprod_subseteq: "x |\<subseteq>| x' \<and> y |\<subseteq>| y' \<Longrightarrow> x |\<times>| y |\<subseteq>| x' |\<times>| y'"
+  apply (simp add: fprod_def less_eq_fset_def Abs_fset_inverse)
+  by auto
+
+lemma fimage_fprod: "(a, b) |\<in>| A |\<times>| B \<Longrightarrow> f a b |\<in>| (\<lambda>(x, y). f x y) |`| (A |\<times>| B)"
+  by force
+
+lemma fprod_singletons: "{|a|} |\<times>| {|b|} = {|(a, b)|}"
+  apply (simp add: fprod_def)
+  by (metis fset_inverse fset_simps(1) fset_simps(2))
+
+lemma fprod_equiv: "(fset (f |\<times>| f') = s) = (((fset f) \<times> (fset f')) = s)"
+  by (simp add: fprod_def Abs_fset_inverse)
+
+lemma fis_singleton_alt: "fis_singleton f = (\<exists>e. f = {|e|})"
+  by (metis fis_singleton.rep_eq fset_inverse fset_simps(1) fset_simps(2) is_singleton_def)
+
+lemma singleton_singleton [simp]: "fis_singleton {|a|}"
+  by (simp add: fis_singleton_def)
+
+lemma not_singleton_empty [simp]: "\<not> fis_singleton {||}"
+  apply (simp add: fis_singleton_def)
+  by (simp add: is_singleton_altdef)
+
+lemma fis_singleton_fthe_elem: "fis_singleton A \<longleftrightarrow> A = {|fthe_elem A|}"
+  by (metis fis_singleton_alt fthe_felem_eq)
 end
