Transition_Lexorder.thy
@@ -7,7 +7,7 @@ begin
 instantiation "transition_ext" :: (linorder) linorder begin
 
 definition less_transition_ext :: "'a::linorder transition_scheme \<Rightarrow> 'a transition_scheme \<Rightarrow> bool" where
-"less_transition_ext t1 t2 = ((Label t1, Arity t1, Guard t1, Outputs t1, Updates t1, more t1) < (Label t2, Arity t2, Guard t2, Outputs t2, Updates t2, more t2))"
+"less_transition_ext t1 t2 = ((Label t1, Arity t1, Guards t1, Outputs t1, Updates t1, more t1) < (Label t2, Arity t2, Guards t2, Outputs t2, Updates t2, more t2))"
 
 definition less_eq_transition_ext :: "'a::linorder transition_scheme \<Rightarrow> 'a transition_scheme \<Rightarrow> bool" where
 "less_eq_transition_ext t1 t2 = (t1 < t2 \<or> t1 = t2)"
