VName.thy
@@ -2,6 +2,12 @@ theory VName
 imports Main
 begin
 
+section\<open>Variables\<close>
+text\<open>Variables can either be inputs or registers. Here we define the vname datatype which allows
+us to write expressions in terms of variables and case match during evaluation. We also make the
+vname datatype a member of linorder such that we can establish a linear order on arithmetic
+expressions and subsequently transitions.\<close>
+
 text_raw\<open>\snip{vnametype}{1}{2}{%\<close>
 datatype vname = I nat | R nat
 text_raw\<open>}%endsnip\<close>
